Soundness.thy
@@ -2,4 +2,20 @@ theory Soundness
   imports Semantics
 begin
 
+lemma triple_rule_parallel:
+  fixes a b :: \<open>('x,'p) action process\<close>
+  assumes
+    \<open>\<lbrace> pa \<rbrace> interp_act a \<lbrace> qa \<rbrace>\<close>
+    \<open>\<lbrace> pb \<rbrace> interp_act b \<lbrace> qb \<rbrace>\<close>
+  shows \<open>\<lbrace> pa \<^emph> pb \<rbrace> interp_act (a \<parallel> b) \<lbrace> qa \<^emph> qb \<rbrace>\<close>
+  using assms
+  sorry
+
+lemma triple_rule_frame:
+  fixes a b :: \<open>('x,'p) action process\<close>
+  assumes \<open>\<lbrace> p \<rbrace> interp_act a \<lbrace> q \<rbrace>\<close>
+  shows \<open>\<lbrace> p \<^emph> r \<rbrace> interp_act a \<lbrace> q \<^emph> r \<rbrace>\<close>
+  using assms
+  sorry
+
 end
